Started specifications for Broken Device
- Start proof that decoding a message is a prefix of the original
- Add stuff about encoding natural numbers

BrokenDevice/broken_device.v
@@ -6,20 +6,23 @@ Import ListNotations.
 Require Extraction.
 
 (** ** Definitions *)
+Module Definitions.
 Inductive bit := B0 | B1.
 
 Definition broken_list := list bool.
 Definition message := list bit.
 Definition packet : Set := bit * bit * bit.
+Definition chunk : Set := bool * bool * bool.
 
 Fixpoint encode_nat (n : nat) : message. Admitted.
 Fixpoint decode_nat (x : message) : nat. Admitted.
 
-Fixpoint count_broken (p : broken_list) := match p with
-  | [] => 0
-  | r :: rest => b2n r + count_broken rest
+Fixpoint bools_to_chunks (p : broken_list) : list chunk :=  match p with
+  | a :: b :: c :: rest => (a,b,c) :: bools_to_chunks rest
+  | _ => []
   end.
 
+Definition sum_chunk '((a,b,c) : chunk) := b2n a + b2n b + b2n c.
 
 Fixpoint packets_to_message (ps : list packet) := match ps with
   | [] => []
@@ -41,49 +44,34 @@ Proof.
   - destruct p as [[a b] c]. simpl. rewrite IH. reflexivity.
 Qed.
 
-Definition encode_packet (a b c : bool) (b1 b2 : bit) : (packet * nat) := 
-    let cnt := b2n a + b2n b + b2n c in
-    match cnt with
-    | 3 => let packet := (match b1, b2 with
+Definition encode_packet '((a,b,c) : chunk) (x : message) : packet := 
+    let '(b1, b2) := (match x with
+      | []                => (B0 , B0)
+      | [b1']             => (b1', B0)
+      | b1' :: b2' :: bs' => (b1', b2')
+    end) in
+    match sum_chunk (a,b,c) with
+    | 0 => (match b1, b2 with
         | B0, B0 => (B0, B1, B1)
         | B0, B1 => (B1, B1, B1)
         | B1, B0 => (B1, B0, B0)
         | B1, B1 => (B1, B0, B1)
-        end) in (packet, 2)
-    | 2 => if negb a then let packet := (match b1 with
+        end)
+    | 1 => if a then (match b1 with
         | B0 => (B0, B0, B1)
         | B1 => (B0, B1, B0)
-        end) in (packet, 1)
-        else if negb c then let packet := (match b1 with
+        end)
+        else if c then (match b1 with
         | B0 => (B1, B1, B0)
         | B1 => (B0, B1, B0)
-        end) in (packet, 1) 
-        else (match b1, b2 with
-        | B0, _  => ((B0, B0, B1), 1)
-        | B1, B0 => ((B1, B0, B0), 2)
-        | B1, B1 => ((B1, B0, B1), 2)
         end)
-    | _ => ((B0, B0, B0), 0)
+        else (match b1, b2 with
+        | B0, _  => (B0, B0, B1)
+        | B1, B0 => (B1, B0, B0)
+        | B1, B1 => (B1, B0, B1)
+        end)
+    | _ => (B0, B0, B0)
     end.
-
-Fixpoint drop {A} (n : nat) (l : list A) : list A := match n, l with
-  | n  , []      => l
-  | 0  , l       => l
-  | S n, x :: ls => drop n ls
-  end.
-
-Fixpoint encode (x : message) (p : broken_list) : list packet := match p with
-  | a :: b :: c :: rest => 
-    let '(b1, b2, bs) := (match x with
-      | []                => (B0 , B0 , [])
-      | [b1']             => (b1', B0 , [])
-      | b1' :: b2' :: bs' => (b1', b2', bs')
-    end) in
-    let '(packet, d) := encode_packet a b c b1 b2 in
-      packet :: encode (drop d x) rest
-  | _ => []
-  end.
-
 
 Definition decode_packet (p : packet) : message := match p with
     | (B0, B0, B0) => []
@@ -96,44 +84,242 @@ Definition decode_packet (p : packet) : message := match p with
     | (B1, B1, B1) => [B0; B1]
     end.
 
+Fixpoint drop {A} (n : nat) (l : list A) : list A := match n, l with
+  | n  , []      => l
+  | 0  , l       => l
+  | S n, x :: ls => drop n ls
+  end.
+
+Fixpoint encode (x : message) (p : list chunk) : list packet := match p with
+  | c :: rest => let pack := encode_packet c x in
+    pack :: encode (drop (length (decode_packet pack)) x) rest
+  | _ => []
+  end.
+
 Fixpoint decode (x : list packet) : message := match x with
   | p :: rest => decode_packet p ++ decode rest
   | _ => []
   end.      
 
 Definition anna (x : message) (p : broken_list) : message :=
-  packets_to_message (encode x p).
+  packets_to_message (encode x (bools_to_chunks p)).
 
 Definition bruno (x : message) : message :=
   decode (message_to_packets x).
+End Definitions.
 
 Module Examples.
-Example ex1 : list packet := encode [B1; B0; B1] [true; true; true; true; true; true; true; true].
-Compute ex1.
-Compute anna [B1; B0; B1] [true; true; true; true; true; true; true; true].
-Compute bruno (anna [B1; B0; B1] [true; true; true; true; true; true; true; true]).
+Import Definitions.
+Definition falses := [false; false; false; false; false; false; false; false; false].
+Compute anna [B1; B0; B1] falses.
+Compute bruno (anna [B1; B0; B1] falses).
 End Examples.
   
 
 (** ** Verification *)
-
-(** Anna's encoding respects the list of broken bits. *)
+Module Verification.
+Import Definitions.
 Inductive matches_broken_list : message -> broken_list -> Prop :=
-  | matches_nil  : 
-      matches_broken_list [] []
+  | matches_nil  : forall p,
+      matches_broken_list [] p
   | matches_true : forall x p,
       matches_broken_list x p ->
       matches_broken_list (B0 :: x) (true :: p)
   | matches_false : forall x p b,
       matches_broken_list x p ->
-      matches_broken_list (b :: x) (true :: p)
-  | matches_extra : forall x p b,
-      matches_broken_list x p ->
-      matches_broken_list x (b :: p).
+      matches_broken_list (b :: x) (false :: p).
+Hint Constructors matches_broken_list : core.
 
-(** This isn't a correct definition, since the decoded message can have extras zeros. *)
-Definition scheme_correct (N K L : nat) := forall (x : message) (p : broken_list), 
-    length p = N ->
-    count_broken p = K ->
-    length x = L -> 
-    decode (encode x p) = x.
+(** A modified induction principle for lists *)
+Theorem list_two_induction {A} (P : list A -> Prop) :
+  P [] -> 
+  (forall a, P [a]) -> 
+  (forall a b l, P l -> 
+                   P (a :: l) -> 
+                   P (a :: b :: l)) ->
+  (forall l, P l).
+Proof.
+  intros H0 H1 IH l.
+  enough (P l /\ (forall a, P (a :: l))) by easy.
+  induction l; intuition. 
+Qed.
+
+Theorem list_three_induction {A} (P : list A -> Prop) :
+  P [] -> 
+  (forall a, P [a]) -> 
+  (forall a b, P [a; b]) -> 
+  (forall a b c l, P l -> 
+                   P (a :: l) -> 
+                   P (a :: b :: l) -> 
+                   P (a :: b :: c :: l)) ->
+  (forall l, P l).
+Proof.
+  intros H0 H1 H2 IH l.
+  enough (P l /\ (forall a, P (a :: l)) /\ (forall a b, P (a :: b :: l))) by easy.
+  induction l; intuition. 
+Qed.
+
+(** Anna's encoding respects the list of broken bits. This can basically be shown by the above induction principle (inducting on groups of threes) and casework. *)
+Theorem anna_respects_broken : forall x p,
+  matches_broken_list (anna x p) p.
+Proof.
+  intros x p.
+  unfold anna.
+  generalize dependent x.
+  induction p as [| | | a b c p IH1 _ _] using list_three_induction; intros; auto.
+  simpl.
+  destruct x as [| x1 x]. 
+    { unfold encode_packet. destruct a, b, c; simpl; auto. } 
+  destruct x as [| x2 x].
+    { destruct x1; unfold encode_packet; destruct a, b, c; simpl; auto. } 
+    { destruct x1, x2, a, b, c; simpl; auto. }
+Qed.
+
+
+(** Two message are equal if they are the same elements, ignoring tailing zeros*)
+(** This definition is still kind of stupid, may adjust it to make the proofs easier *)
+Inductive equal_message : message -> message -> Prop :=
+  | equal_nil : 
+      equal_message [] []
+  | equal_cons : forall xs ys x y,
+      equal_message xs ys ->
+      equal_message (x :: xs) (y :: ys)
+  | equal_tail_0 : forall xs ys,
+      equal_message xs ys ->
+      equal_message xs (ys ++ [B0])
+  | equal_symm : forall xs ys,
+      equal_message xs ys ->
+      equal_message ys xs.
+Hint Constructors equal_message : core.
+
+Example equal_ex : equal_message [B1; B0; B1] [B1; B0; B1; B0; B0; B0].
+Proof.
+  assert (H : [B1; B0; B1; B0; B0; B0] = (([B1; B0; B1] ++ [B0]) ++ [B0]) ++ [B0]).
+  auto.
+  rewrite H.
+  repeat apply equal_tail_0.
+  auto.
+Qed.
+
+Fixpoint count_broken (p : list chunk) := match p with
+  | c :: rest => sum_chunk c + count_broken rest
+  | _ => 0
+  end.
+
+(** Encoding a message [B0] is the same as encoding nothing. May adapt as needed. *)
+Lemma encode_B0 : forall l, encode [B0] l = encode [] l.
+Proof.
+  intros.
+  induction l.
+  simpl. auto.
+  destruct a as [[a b] c].
+  destruct a, b, c; simpl; try rewrite IHl; auto.
+Qed.
+
+(** The number of bits transmitted in a packet depends on the number of true (broken) bits in the chunk. *)
+Lemma number_of_bits_in_packet: forall c msg,
+  length (decode_packet (encode_packet c msg)) >= 2 - (sum_chunk c).
+Proof.
+  intros [[a b] c] [| [|] [| [|] x]]; destruct a, b, c; simpl; auto.
+Qed.
+  
+(** chunk_count records the number of chunks in a list with count 0, 1, 2/3*)
+Inductive chunk_count : list chunk -> nat -> nat -> nat -> Prop :=
+  | cc_nil : chunk_count [] 0 0 0
+  | cc_0   : forall l x y z c,
+      sum_chunk c = 0 ->
+      chunk_count l x y z ->
+      chunk_count (c::l) (S x) y z
+  | cc_1   : forall l x y z c,
+      sum_chunk c = 1 ->
+      chunk_count l x y z ->
+      chunk_count (c::l) x (S y) z
+  | cc_2_or_3   : forall l x y z c,
+      sum_chunk c = 2 \/ sum_chunk c = 3 ->
+      chunk_count l x y z ->
+      chunk_count (c::l) x y (S z).
+Hint Constructors chunk_count : core.
+
+Lemma list_to_chunk_count : forall (l : list chunk),
+    exists x y z, chunk_count l x y z.
+Proof.
+  intros.
+  induction l; eauto.
+  remember (sum_chunk a) as sum.
+  destruct IHl as [x [y [z IHl]]].
+  destruct a as [[a b] c].
+  destruct a, b, c; pose proof Heqsum as H; simpl in H;
+  repeat eexists; match goal with 
+    | [ _ : sum = 0 |- _] => apply cc_0
+    | [ _ : sum = 1 |- _] => apply cc_1
+    | [ _ : sum = 2 |- _] => apply cc_2_or_3
+    | [ _ : sum = 3 |- _] => apply cc_2_or_3
+  end; simpl; try lia; apply IHl.
+Qed.
+
+Lemma chunk_count_total : forall l x y z,
+  chunk_count l x y z ->
+  x + y + z = length l.
+Proof.
+  intros. induction H; simpl; lia.
+Qed.
+
+Lemma chunk_count_sumsto_count_broken : forall l x y z,
+  chunk_count l x y z -> 
+  y + 2*z <= count_broken l.
+Proof.
+  intros. induction H; simpl; try rewrite H; lia.
+Qed.  
+
+Lemma chunk_count_decoded_length : forall msg l x y z,
+  chunk_count l x y z ->
+  length (decode (encode msg l)) >= 2*x + y.
+Proof.
+  intros.
+  generalize dependent msg.
+  induction H; intros; try (simpl; lia); simpl;
+    rewrite app_length;
+    remember (encode_packet c msg) as ep;
+    pose proof (number_of_bits_in_packet c msg); rewrite <- Heqep in H1;
+    specialize IHchunk_count with (drop (length (decode_packet ep)) msg); lia.
+Qed.
+
+Definition message_preserved (N K L : nat) := forall x p, 
+  length p = N ->
+  count_broken (bools_to_chunks p) = K ->
+  length x = L ->
+  equal_message (bruno (anna x p)) x.
+
+Lemma bools_to_chunks_length : forall p (m n : nat),
+  length p = n ->
+  3 * m = n ->
+  length (bools_to_chunks p) = m.
+Proof.
+  intros.
+  generalize dependent n.
+  generalize dependent m.
+  induction p using list_three_induction; intros; simpl in *; auto; try lia.
+  clear IHp0. clear IHp1.
+  rewrite (IHp (m-1) (n-3)); lia. 
+Qed.
+
+Theorem correct_message_for_given_constraints :
+  message_preserved 150 40 60.
+Proof.
+  unfold message_preserved.
+  intros msg p H1 H2 H3.
+  unfold bruno, anna. rewrite packets_message_inverses.
+  remember (bools_to_chunks p) as l.
+  destruct (list_to_chunk_count l) as [x [y [z Hcnt]]].
+  assert (xy_lb : 2*x + y >= 60). { 
+    assert (Hp_length : length l = 50). { subst. apply bools_to_chunks_length with (n := 150); auto. }
+    pose proof (chunk_count_total l x y z Hcnt).
+    pose proof (chunk_count_sumsto_count_broken l x y z Hcnt).
+    lia. }
+  pose proof (chunk_count_decoded_length msg l x y z Hcnt) as H_decoded_length.
+  (* Now we know that the length of the decoded message is at least 60 (the length of the original message). *)
+  (* Next, we must show that any decoded message is either a prefix of the original message, or it is equal (possibly with tailing zeros). 
+     Since we know that it cannot be a strict prefix since its length is >= 60, it must indeed be equal. *)
+Admitted.  
+
+End Verification.
